fv: package instance objects and theorems into formal instance

fv/lean/Ragu/Instances/Point/Alloc.lean
@@ -5,29 +5,32 @@ namespace Ragu.Instances.Point.Alloc
 open Core.Primes
 
 @[reducible]
-def CircuitField := F Core.Primes.p
+def p := Core.Primes.p
 
-def Inputs := unit
+@[reducible]
+def inputLen := 0
 
--- Point allocation instance:
+@[reducible]
+def outputLen := 2
+
 set_option linter.unusedVariables false in
-def exported_operations (input_var : Var Inputs CircuitField) : Operations CircuitField := [
+def exportedOperations (input_var : Var (ProvableVector field inputLen) (F Core.Primes.p)) : Operations (F p) := [
   Operation.witness 3 (fun _env => default),
-  Operation.assert ((((var 0) * (var 1)) + ((0x40000000000000000000000000000000224698fc094cf91b992d30ed00000000 : Expression CircuitField) * (var 2)))),
-  Operation.assert (((var 0) + ((0x40000000000000000000000000000000224698fc094cf91b992d30ed00000000 : Expression CircuitField) * (var 1)))),
+  Operation.assert ((((var 0) * (var 1)) + ((0x40000000000000000000000000000000224698fc094cf91b992d30ed00000000 : Expression (F p)) * (var 2)))),
+  Operation.assert (((var 0) + ((0x40000000000000000000000000000000224698fc094cf91b992d30ed00000000 : Expression (F p)) * (var 1)))),
   Operation.witness 3 (fun _env => default),
-  Operation.assert ((((var 3) * (var 4)) + ((0x40000000000000000000000000000000224698fc094cf91b992d30ed00000000 : Expression CircuitField) * (var 5)))),
-  Operation.assert (((var 3) + ((0x40000000000000000000000000000000224698fc094cf91b992d30ed00000000 : Expression CircuitField) * (var 0)))),
-  Operation.assert (((var 4) + ((0x40000000000000000000000000000000224698fc094cf91b992d30ed00000000 : Expression CircuitField) * (var 2)))),
+  Operation.assert ((((var 3) * (var 4)) + ((0x40000000000000000000000000000000224698fc094cf91b992d30ed00000000 : Expression (F p)) * (var 5)))),
+  Operation.assert (((var 3) + ((0x40000000000000000000000000000000224698fc094cf91b992d30ed00000000 : Expression (F p)) * (var 0)))),
+  Operation.assert (((var 4) + ((0x40000000000000000000000000000000224698fc094cf91b992d30ed00000000 : Expression (F p)) * (var 2)))),
   Operation.witness 3 (fun _env => default),
-  Operation.assert ((((var 6) * (var 7)) + ((0x40000000000000000000000000000000224698fc094cf91b992d30ed00000000 : Expression CircuitField) * (var 8)))),
-  Operation.assert (((var 6) + ((0x40000000000000000000000000000000224698fc094cf91b992d30ed00000000 : Expression CircuitField) * (var 7)))),
-  Operation.assert ((((var 5) + ((0x0000000000000000000000000000000000000000000000000000000000000005 : Expression CircuitField) * 1)) + ((0x40000000000000000000000000000000224698fc094cf91b992d30ed00000000 : Expression CircuitField) * (var 8)))),
+  Operation.assert ((((var 6) * (var 7)) + ((0x40000000000000000000000000000000224698fc094cf91b992d30ed00000000 : Expression (F p)) * (var 8)))),
+  Operation.assert (((var 6) + ((0x40000000000000000000000000000000224698fc094cf91b992d30ed00000000 : Expression (F p)) * (var 7)))),
+  Operation.assert ((((var 5) + ((0x0000000000000000000000000000000000000000000000000000000000000005 : Expression (F p)) * 1)) + ((0x40000000000000000000000000000000224698fc094cf91b992d30ed00000000 : Expression (F p)) * (var 8)))),
 ]
 
 set_option linter.unusedVariables false in
 @[reducible]
-def exported_output (input_var : Var Inputs CircuitField) : Vector (Expression CircuitField) 2 := #v[
+def exportedOutput (input_var : Var (ProvableVector field inputLen) (F Core.Primes.p)) : Vector (Expression (F p)) outputLen := #v[
   (var 0),
   (var 6)
 ]
@@ -35,33 +38,42 @@ def exported_output (input_var : Var Inputs CircuitField) : Vector (Expression C
 def circuit := Circuits.Point.Alloc.circuit Circuits.Point.Spec.EpAffineParams (p:=Core.Primes.p)
 
 set_option linter.unusedVariables false in
-def deserializeInput (input : Var Inputs CircuitField) : Var unit CircuitField := ()
+def deserializeInput (input : Var (ProvableVector field inputLen) (F p)) : Var unit (F p) := ()
 
-def serializeOutput (output: Var Circuits.Point.Spec.Point CircuitField) : Vector (Expression CircuitField) 2 :=
+def serializeOutput (output: Var Circuits.Point.Spec.Point (F p)) : Vector (Expression (F p)) outputLen :=
   #v[
     output.x,
     output.y
   ]
 
-theorem same_circuit (input : Var Inputs CircuitField):
-    ((circuit input).operations 0).toFlat = (exported_operations input).toFlat := by
-  simp [Operations.toFlat, circuit_norm, FormalCircuit.toSubcircuit,
-    circuit,
-    Circuits.Point.Alloc.circuit, Circuits.Point.Alloc.elaborated, Circuits.Point.Alloc.main,
-    Circuits.Core.AllocMul.circuit, Circuits.Core.AllocMul.elaborated, Circuits.Core.AllocMul.main,
-    Circuits.Element.AllocSquare.circuit, Circuits.Element.AllocSquare.elaborated, Circuits.Element.AllocSquare.main,
-    Circuits.Element.Mul.circuit, Circuits.Element.Mul.elaborated, Circuits.Element.Mul.main]
-  rfl
+def formal_instance : Core.Statements.FormalInstance where
+  p
+  inputLen
+  outputLen
+  exportedOperations
+  exportedOutput
 
-theorem same_output (input : Var Inputs CircuitField) :
-  ((deserializeInput input) |> circuit |>.output 0 |> serializeOutput) = exported_output input:= by
-  simp [circuit_norm,
-    circuit, serializeOutput,
-    Circuits.Point.Alloc.circuit, Circuits.Point.Alloc.elaborated, Circuits.Point.Alloc.main,
-    Circuits.Core.AllocMul.circuit, Circuits.Core.AllocMul.elaborated, Circuits.Core.AllocMul.main,
-    Circuits.Element.AllocSquare.circuit, Circuits.Element.AllocSquare.elaborated, Circuits.Element.AllocSquare.main,
-    Circuits.Element.Mul.circuit, Circuits.Element.Mul.elaborated, Circuits.Element.Mul.main]
-  constructor <;> rfl
+  Input := unit
+  Output := Circuits.Point.Spec.Point
 
+  deserializeInput
+  serializeOutput
+
+  Assumptions input := True
+  Spec input output := output.isOnCurve Circuits.Point.Spec.EpAffineParams
+
+  reimplementation := Circuits.Point.Alloc.circuit Circuits.Point.Spec.EpAffineParams
+
+  same_circuit := by
+    intro input
+    simp [Operations.toFlat, circuit_norm, FormalCircuit.toSubcircuit,
+      Circuits.Point.Alloc.circuit, Circuits.Point.Alloc.elaborated, Circuits.Point.Alloc.main,
+      Circuits.Core.AllocMul.circuit, Circuits.Core.AllocMul.elaborated, Circuits.Core.AllocMul.main,
+      Circuits.Element.AllocSquare.circuit, Circuits.Element.AllocSquare.elaborated, Circuits.Element.AllocSquare.main,
+      Circuits.Element.Mul.circuit, Circuits.Element.Mul.elaborated, Circuits.Element.Mul.main]
+    rfl
+  same_output := by intro input; rfl
+  same_spec := by intro input output; rfl
+  same_assumptions := by intro input; rfl
 
 end Ragu.Instances.Point.Alloc
